Refactor project into a more common Lean layout

LeanMqtt/Core/Parser.lean
@@ -1,5 +1,0 @@
-abbrev Parser (α : Type) := StateT (List UInt8) Option α
-
-theorem parser_app_is_run {α} {l : List UInt8} (p : Parser α) :
-  p l = p.run l :=
-  rfl
