LeanMqtt/Packets/VarHeader/Variations.lean
@@ -1,10 +1,16 @@
-import LeanMqtt.Core.Parser
-import LeanMqtt.Defs.Packets.VarHeader
-import LeanMqtt.Serialization.Packets.Properties
-import LeanMqtt.Serialization.Primitives
+import LeanMqtt.Primitives.Basic
+import LeanMqtt.Packets.VarHeader.Properties
 
 namespace Mqtt
 open Mqtt
+
+/- ========================= Var_Connect ========================= -/
+
+structure Var_Connect where
+  protocol_name    : Str
+  protocol_version : UInt8
+  connect_flags    : UInt8
+  props            : Properties
 
 def Var_Connect.serialize (v : Var_Connect) : List UInt8 :=
   v.protocol_name.serialize ++
@@ -19,6 +25,13 @@ def Var_Connect.parser : Parser Var_Connect := do
   let props ← Properties.parser
   return { protocol_name, protocol_version, connect_flags, props }
 
+/- ========================= Var_Connack ========================= -/
+
+structure Var_Connack where
+  ack_flags   : UInt8
+  reason_code : UInt8
+  props       : Properties
+
 def Var_Connack.serialize (v : Var_Connack) : List UInt8 :=
   v.ack_flags.serialize ++
   v.reason_code.serialize ++
@@ -29,6 +42,13 @@ def Var_Connack.parser : Parser Var_Connack := do
   let reason_code ← UInt8.parser
   let props       ← Properties.parser
   return { ack_flags, reason_code, props }
+
+/- ========================= Var_Publish ========================= -/
+
+structure Var_Publish (qos : BitVec 2) where
+  topic_name : Str
+  packet_id  : if qos > 0 then UInt16 else Unit
+  props      : Properties
 
 def Var_Publish.serialize {qos} (v : Var_Publish qos) : List UInt8 :=
   v.topic_name.serialize ++
@@ -53,6 +73,14 @@ def Var_Publish.parser (qos : BitVec 2) : Parser (Var_Publish qos) := do
 
   return { topic_name, packet_id, props }
 
+/- ========================= Var_Puback ========================= -/
+
+structure Var_Puback where
+  packet_id   : UInt16
+  reason_code : UInt8
+  -- TODO: dependent on remaining length
+  props       : Properties
+
 def Var_Puback.serialize (v : Var_Puback) : List UInt8 :=
   v.packet_id.serialize ++
   v.reason_code.serialize ++
@@ -63,6 +91,14 @@ def Var_Puback.parser : Parser (Var_Puback) := do
   let reason_code ← UInt8.parser
   let props ← Properties.parser
   return { packet_id, reason_code, props }
+
+/- ========================= Var_Pubrec ========================= -/
+
+structure Var_Pubrec where
+  packet_id   : UInt16
+  reason_code : UInt8
+  -- TODO: dependent on remaining length
+  props       : Properties
 
 def Var_Pubrec.serialize (v : Var_Pubrec) : List UInt8 :=
   v.packet_id.serialize ++
@@ -75,6 +111,13 @@ def Var_Pubrec.parser : Parser (Var_Pubrec) := do
   let props ← Properties.parser
   return { packet_id, reason_code, props }
 
+/- ========================= Var_Pubrel ========================= -/
+
+structure Var_Pubrel where
+  packet_id   : UInt16
+  reason_code : UInt8
+  props       : Properties
+
 def Var_Pubrel.serialize (v : Var_Pubrel) : List UInt8 :=
   v.packet_id.serialize ++
   v.reason_code.serialize ++
@@ -85,6 +128,13 @@ def Var_Pubrel.parser : Parser (Var_Pubrel) := do
   let reason_code ← UInt8.parser
   let props ← Properties.parser
   return { packet_id, reason_code, props }
+
+/- ========================= Var_Pubcomp ========================= -/
+
+structure Var_Pubcomp where
+  packet_id   : UInt16
+  reason_code : UInt8
+  props       : Properties
 
 def Var_Pubcomp.serialize (v : Var_Pubcomp) : List UInt8 :=
   v.packet_id.serialize ++
@@ -97,6 +147,12 @@ def Var_Pubcomp.parser : Parser (Var_Pubcomp) := do
   let props ← Properties.parser
   return { packet_id, reason_code, props }
 
+/- ========================= Var_Subscribe ========================= -/
+
+structure Var_Subscribe where
+  packet_id : UInt16
+  props     : Properties
+
 def Var_Subscribe.serialize (v : Var_Subscribe) : List UInt8 :=
   v.packet_id.serialize ++
   v.props.serialize
@@ -105,6 +161,12 @@ def Var_Subscribe.parser : Parser (Var_Subscribe) := do
   let packet_id ← UInt16.parser
   let props ← Properties.parser
   return { packet_id, props }
+
+/- ========================= Var_Suback ========================= -/
+
+structure Var_Suback where
+  packet_id : UInt16
+  props     : Properties
 
 def Var_Suback.serialize (v : Var_Suback) : List UInt8 :=
   v.packet_id.serialize ++
@@ -115,6 +177,12 @@ def Var_Suback.parser : Parser (Var_Suback) := do
   let props ← Properties.parser
   return { packet_id, props }
 
+/- ========================= Var_Unsubscribe ========================= -/
+
+structure Var_Unsubscribe where
+  packet_id : UInt16
+  props     : Properties
+
 def Var_Unsubscribe.serialize (v : Var_Unsubscribe) : List UInt8 :=
   v.packet_id.serialize ++
   v.props.serialize
@@ -123,6 +191,12 @@ def Var_Unsubscribe.parser : Parser (Var_Unsubscribe) := do
   let packet_id ← UInt16.parser
   let props ← Properties.parser
   return { packet_id, props }
+
+/- ========================= Var_Unsuback ========================= -/
+
+structure Var_Unsuback where
+  packet_id : UInt16
+  props     : Properties
 
 def Var_Unsuback.serialize (v : Var_Unsuback) : List UInt8 :=
   v.packet_id.serialize ++
@@ -133,11 +207,25 @@ def Var_Unsuback.parser : Parser (Var_Unsuback) := do
   let props ← Properties.parser
   return { packet_id, props }
 
+/- ========================= Var_Pingreq ========================= -/
+
+abbrev Var_Pingreq  := Unit
+
 def Var_Pingreq.serialize (_ : Var_Pingreq) : List UInt8 := []
 def Var_Pingreq.parser : Parser (Var_Pingreq) := return ()
 
+/- ========================= Var_Pingresp ========================= -/
+
+abbrev Var_Pingresp := Unit
+
 def Var_Pingresp.serialize (_ : Var_Pingresp) : List UInt8 := []
 def Var_Pingresp.parser : Parser (Var_Pingresp) := return ()
+
+/- ========================= Var_Disconnect ========================= -/
+
+structure Var_Disconnect where
+  reason_code : UInt8
+  props       : Properties
 
 def Var_Disconnect.serialize (v : Var_Disconnect) : List UInt8 :=
   v.reason_code.serialize ++
@@ -148,6 +236,12 @@ def Var_Disconnect.parser : Parser (Var_Disconnect) := do
   let props ← Properties.parser
   return { reason_code, props }
 
+/- ========================= Var_Auth ========================= -/
+
+structure Var_Auth where
+  reason_code : UInt8
+  props       : Properties
+
 def Var_Auth.serialize (v : Var_Auth) : List UInt8 :=
   v.reason_code.serialize ++
   v.props.serialize
@@ -156,48 +250,5 @@ def Var_Auth.parser : Parser (Var_Auth) := do
   let reason_code ← UInt8.parser
   let props ← Properties.parser
   return { reason_code, props }
-
-def VarHeader.serializeValue {w : WhichPkt} {f : WhichPkt.flagType w}
-  (v : VarHeader.getType w f) : List UInt8 :=
-  match w with
-  | .connect     => Var_Connect.serialize v
-  | .connack     => Var_Connack.serialize v
-  | .publish     => @Var_Publish.serialize f.qos v
-  | .puback      => Var_Puback.serialize v
-  | .pubrec      => Var_Pubrec.serialize v
-  | .pubrel      => Var_Pubrel.serialize v
-  | .pubcomp     => Var_Pubcomp.serialize v
-  | .subscribe   => Var_Subscribe.serialize v
-  | .suback      => Var_Suback.serialize v
-  | .unsubscribe => Var_Unsubscribe.serialize v
-  | .unsuback    => Var_Unsuback.serialize v
-  | .pingreq     => Var_Pingreq.serialize v
-  | .pingresp    => Var_Pingresp.serialize v
-  | .disconnect  => Var_Disconnect.serialize v
-  | .auth        => Var_Auth.serialize v
-
-def VarHeader.parserValue (w : WhichPkt) (f : WhichPkt.flagType w) : Parser (VarHeader.getType w f) :=
-  match w with
-  | .connect     => Var_Connect.parser
-  | .connack     => Var_Connack.parser
-  | .publish     => Var_Publish.parser f.qos
-  | .puback      => Var_Puback.parser
-  | .pubrec      => Var_Pubrec.parser
-  | .pubrel      => Var_Pubrel.parser
-  | .pubcomp     => Var_Pubcomp.parser
-  | .subscribe   => Var_Subscribe.parser
-  | .suback      => Var_Suback.parser
-  | .unsubscribe => Var_Unsubscribe.parser
-  | .unsuback    => Var_Unsuback.parser
-  | .pingreq     => Var_Pingreq.parser
-  | .pingresp    => Var_Pingresp.parser
-  | .disconnect  => Var_Disconnect.parser
-  | .auth        => Var_Auth.parser
-
-def VarHeader.serialize (h : FixedHeader) (v : VarHeader h) : List UInt8 :=
-  VarHeader.serializeValue v
-
-def VarHeader.parser (h : FixedHeader) : Parser (VarHeader h) :=
-  VarHeader.parserValue h.which h.flags
 
 end Mqtt
