LeanMqtt.lean
@@ -1,5 +1,4 @@
 -- This module serves as the root of the `LeanMqtt` library.
 -- Import modules here that should be built as part of the library.
-import LeanMqtt.Defs.Packets.Packet
-import LeanMqtt.Serialization.Packets.Packet
-import LeanMqtt.Proofs.Packets.Packet
+import LeanMqtt.Packets.Packet.Basic
+import LeanMqtt.Packets.Packet.Proofs
