LeanMqtt/Core/Parser/Basic.lean
@@ -1,0 +1,28 @@
+abbrev Parser (α : Type) := StateT (List UInt8) Option α
+
+theorem parser_app_is_run {α} {l : List UInt8} (p : Parser α) :
+  p l = p.run l :=
+  rfl
+
+def bytesParser (n : Nat) : Parser (List UInt8) := do
+  let s ← get
+  if s.length < n then
+    none
+  else
+    let chunk := s.take n
+    let rest  := s.drop n
+    set rest
+    return chunk
+
+def bytesParserWithProof (n : Nat) : Parser { l : List UInt8 // l.length = n } := do
+  let s ← get
+  if h : s.length < n then
+    none
+  else
+    let chunk := s.take n
+    let rest  := s.drop n
+    set rest
+    -- Prove that the chunk has the correct length
+    have h_len : chunk.length = n :=
+      List.length_take_of_le (Nat.ge_of_not_lt h)
+    return ⟨chunk, h_len⟩
