LeanMqtt/Core/Parser/Proofs.lean
@@ -1,0 +1,65 @@
+import LeanMqtt.Core.Parser.Basic
+
+theorem bytesParser_len (n : Nat) (l inp rest : List UInt8) :
+  (bytesParser n).run inp = some (l, rest) → l.length = n := by
+  simp [bytesParser]
+  split
+  · intro h_len
+    contradiction
+  · next h_len =>
+    intro h
+    simp at h
+    have ⟨h_l, h_rest⟩ := h
+    subst h_l
+    simp [List.length_take]
+    omega
+
+theorem bytesParser_reconstruct (n : Nat) (input : List UInt8) (chunk rest : List UInt8) :
+  (bytesParser n).run input = some (chunk, rest) → input = chunk ++ rest := by
+  simp [bytesParser]
+  split
+  · intro; contradiction
+  · next h_len =>
+    simp
+    intro h1 h2
+    rw [←h1, ←h2]
+    apply Eq.symm
+    apply List.take_append_drop n input
+
+theorem roundtrip_bytes (l : List UInt8) (rest : List UInt8) :
+  (bytesParser l.length).run (l ++ rest) = some (l, rest) := by
+  simp [bytesParser]
+  split
+  · omega
+  · simp
+
+theorem roundtrip_bytes_with_proof (l : List UInt8) (rest : List UInt8) :
+  (bytesParserWithProof l.length).run (l ++ rest) = some (⟨l, rfl⟩, rest) := by
+  simp [bytesParserWithProof]
+  split
+  · omega
+  · simp
+
+theorem bytesParserWithProof_eq_parser_success (n : Nat)
+  (l : List UInt8) (inp rest : List UInt8) :
+  (bytesParser n).run inp = some (l, rest) →
+  ∃ h, (bytesParserWithProof n).run inp = some (⟨l, h⟩, rest) := by
+  intro h_simple
+  have h_len_parser := bytesParser_len _ _ _ _ h_simple
+  simp only [bytesParser, bytesParserWithProof] at *
+  simp only [bind_pure_comp, StateT.run_bind, StateT.run_get,
+    Option.pure_def, Option.bind_eq_bind, Option.bind_some
+  ] at *
+  split at h_simple
+  · contradiction
+  · next h_len =>
+    simp only [StateT.run_map, StateT.run_set, Option.pure_def,
+      Option.map_eq_map, Option.map_some, Option.some.injEq, Prod.mk.injEq
+    ] at h_simple
+    simp only [dif_neg h_len]
+    simp only [StateT.run_map, StateT.run_set, Option.pure_def,
+      Option.map_eq_map, Option.map_some, Option.some.injEq, Prod.mk.injEq,
+      Subtype.mk.injEq, exists_and_left, exists_prop
+    ]
+    rcases h_simple with ⟨h_take, h_drop⟩
+    exact ⟨h_take, h_len_parser, h_drop⟩
