LeanMqtt/Packets/FixedHeader/Basic.lean
@@ -1,13 +1,52 @@
-import LeanMqtt.Core.Parser
-import LeanMqtt.Defs.Packets.FixedHeader
-import LeanMqtt.Serialization.Primitives
-
-private instance (r : Std.Range) (i : Nat) : Decidable (i ∈ r) := by
-  dsimp [Membership.mem]
-  infer_instance
+import LeanMqtt.Primitives.Basic
 
 namespace Mqtt
 open Mqtt
+
+/- ========================= WhichPkt ========================= -/
+
+inductive WhichPkt where
+  | connect
+  | connack
+  | publish
+  | puback
+  | pubrec
+  | pubrel
+  | pubcomp
+  | subscribe
+  | suback
+  | unsubscribe
+  | unsuback
+  | pingreq
+  | pingresp
+  | disconnect
+  | auth
+deriving Repr, BEq
+
+instance : Inhabited WhichPkt where
+  default := .pingreq
+
+structure PublishFlags where
+  dup : BitVec 1
+  qos : BitVec 2
+  retain : BitVec 1
+
+def WhichPkt.flagType : WhichPkt → Type
+  | .connect     => { i : BitVec 4 // i = 0b0000 }
+  | .connack     => { i : BitVec 4 // i = 0b0000 }
+  | .publish     => PublishFlags
+  | .puback      => { i : BitVec 4 // i = 0b0000 }
+  | .pubrec      => { i : BitVec 4 // i = 0b0000 }
+  | .pubrel      => { i : BitVec 4 // i = 0b0010 }
+  | .pubcomp     => { i : BitVec 4 // i = 0b0000 }
+  | .subscribe   => { i : BitVec 4 // i = 0b0010 }
+  | .suback      => { i : BitVec 4 // i = 0b0000 }
+  | .unsubscribe => { i : BitVec 4 // i = 0b0010 }
+  | .unsuback    => { i : BitVec 4 // i = 0b0000 }
+  | .pingreq     => { i : BitVec 4 // i = 0b0000 }
+  | .pingresp    => { i : BitVec 4 // i = 0b0000 }
+  | .disconnect  => { i : BitVec 4 // i = 0b0000 }
+  | .auth        => { i : BitVec 4 // i = 0b0000 }
 
 def WhichPkt.encode (pkt : WhichPkt) : BitVec 4 :=
   match pkt with
@@ -97,6 +136,14 @@ def WhichPkt.parser : Parser ((which : WhichPkt) × WhichPkt.flagType which) := 
   let which ← WhichPkt.decode? whichBits
   let flags ← WhichPkt.decodeFlags which flagsBits
   return ⟨which, flags⟩
+
+/- ========================= FixedHeader ========================= -/
+
+structure FixedHeader where
+  which : WhichPkt
+  flags : WhichPkt.flagType which
+  size  : VarInt -- TODO: depend on information after
+
 
 def FixedHeader.serialize : FixedHeader → List UInt8 :=
   fun ⟨which, flags, size⟩ =>
