LeanMqtt/Packets/Packet/Basic.lean
@@ -1,0 +1,25 @@
+import LeanMqtt.Packets.FixedHeader.Basic
+import LeanMqtt.Packets.VarHeader.Basic
+import LeanMqtt.Packets.Payload.Basic
+
+namespace Mqtt
+
+structure Header where
+  fix : FixedHeader
+  var : VarHeader fix
+
+def Header.serialize (h : Header) : List UInt8 :=
+  FixedHeader.serialize h.fix ++
+  VarHeader.serialize h.fix h.var
+
+def Header.parser : Parser Header := do
+  let fix ← FixedHeader.parser
+  let var ← VarHeader.parser fix
+  return { fix, var }
+
+structure Packet where
+  fixed_header : FixedHeader
+  var_header   : VarHeader fixed_header
+  payload      : Payload
+
+end Mqtt
