LeanMqtt/Packets/VarHeader/Basic.lean
@@ -1,0 +1,79 @@
+import LeanMqtt.Primitives.Basic
+import LeanMqtt.Packets.FixedHeader.Basic
+import LeanMqtt.Packets.VarHeader.Properties
+import LeanMqtt.Packets.VarHeader.Variations
+
+namespace Mqtt
+open Mqtt
+
+/- ========================= VarHeader ========================= -/
+
+/--
+  Determines the Variable Header type based on the Packet Kind
+  and the specific flags (needed for Publish QoS).
+-/
+def VarHeader.getType (w : WhichPkt) (f : WhichPkt.flagType w) : Type :=
+  match w with
+  | .connect     => Var_Connect
+  | .connack     => Var_Connack
+  | .publish     => Var_Publish f.qos
+  | .puback      => Var_Puback
+  | .pubrec      => Var_Pubrec
+  | .pubrel      => Var_Pubrel
+  | .pubcomp     => Var_Pubcomp
+  | .subscribe   => Var_Subscribe
+  | .suback      => Var_Suback
+  | .unsubscribe => Var_Unsubscribe
+  | .unsuback    => Var_Unsuback
+  | .pingreq     => Var_Pingreq
+  | .pingresp    => Var_Pingresp
+  | .disconnect  => Var_Disconnect
+  | .auth        => Var_Auth
+
+def VarHeader.serializeValue {w : WhichPkt} {f : WhichPkt.flagType w}
+  (v : VarHeader.getType w f) : List UInt8 :=
+  match w with
+  | .connect     => Var_Connect.serialize v
+  | .connack     => Var_Connack.serialize v
+  | .publish     => @Var_Publish.serialize f.qos v
+  | .puback      => Var_Puback.serialize v
+  | .pubrec      => Var_Pubrec.serialize v
+  | .pubrel      => Var_Pubrel.serialize v
+  | .pubcomp     => Var_Pubcomp.serialize v
+  | .subscribe   => Var_Subscribe.serialize v
+  | .suback      => Var_Suback.serialize v
+  | .unsubscribe => Var_Unsubscribe.serialize v
+  | .unsuback    => Var_Unsuback.serialize v
+  | .pingreq     => Var_Pingreq.serialize v
+  | .pingresp    => Var_Pingresp.serialize v
+  | .disconnect  => Var_Disconnect.serialize v
+  | .auth        => Var_Auth.serialize v
+
+def VarHeader.parserValue (w : WhichPkt) (f : WhichPkt.flagType w) : Parser (VarHeader.getType w f) :=
+  match w with
+  | .connect     => Var_Connect.parser
+  | .connack     => Var_Connack.parser
+  | .publish     => Var_Publish.parser f.qos
+  | .puback      => Var_Puback.parser
+  | .pubrec      => Var_Pubrec.parser
+  | .pubrel      => Var_Pubrel.parser
+  | .pubcomp     => Var_Pubcomp.parser
+  | .subscribe   => Var_Subscribe.parser
+  | .suback      => Var_Suback.parser
+  | .unsubscribe => Var_Unsubscribe.parser
+  | .unsuback    => Var_Unsuback.parser
+  | .pingreq     => Var_Pingreq.parser
+  | .pingresp    => Var_Pingresp.parser
+  | .disconnect  => Var_Disconnect.parser
+  | .auth        => Var_Auth.parser
+
+abbrev VarHeader (h : FixedHeader) : Type :=
+  VarHeader.getType h.which h.flags
+
+def VarHeader.serialize (h : FixedHeader) (v : VarHeader h) : List UInt8 :=
+  VarHeader.serializeValue v
+
+def VarHeader.parser (h : FixedHeader) : Parser (VarHeader h) :=
+  VarHeader.parserValue h.which h.flags
+
+end Mqtt
